\section*{Introduction}
\textbf{\large 1. Use Euler's formula to prove that:}

\begin{equation*}
	\sin(x) \cos(x) = \frac{1}{2} \sin(2x)
\end{equation*}

\textbf{Given that:}

\begin{align}
	e^{ix} &= \cos(x) + i \sin(x) \label{eq:1}\\
	e^{-ix} &= \cos(-x) + i \sin(-x) = \cos(x) - i \sin(x) \label{eq:2}
\end{align}

\textbf{Follows:}

\begin{align}
	\cos(x) &= \frac{e^{ix} + e^{-ix}}{2} & & \text{Added \eqref{eq:1} and \eqref{eq:2}} \label{eq:3}\\
	\sin(x) &= \frac{e^{ix} - e^{-ix}}{2i} & & \text{Subtracted \eqref{eq:1} from \eqref{eq:2}} \label{eq:4}
\end{align}

\begin{align*}
	\sin(x) \cos(x) &= \frac{e^{ix} + e^{-ix}}{2} \cdot \frac{e^{ix} - e^{-ix}}{2i} & & \text{Substituting \eqref{eq:3} and \eqref{eq:4}}\\
	&= \frac{e^{i2x} - e^{i0} + e^{i0} - e^{-i2x}}{4i} & & \text{Multiplied fractions}\\
	&= \frac{1}{2} \frac{e^{i2x} - e^{-i2x}}{2i} & & \text{Combined exponentials}\\
	&= \frac{1}{2} \sin(2x) & & \text{Substituted \eqref{eq:4}}
\end{align*}

\textbf{\large 2. Show that:}

\begin{equation*}
	\int_0^{T_0} \cos(k \omega_0 t) \cos(n \omega_0 t) dt =
	\begin{cases}
		0,& k \neq n\\
		\frac{T_0}{2},& k = n \neq 0\\
		T_0,& k = n = 0
	\end{cases}
\end{equation*}

\textbf{Given that:}

\begin{equation}
	\cos(x) \cos(y) = \frac{1}{2} \left[ \cos(x-y) + cos(x+y) \right]
\end{equation}

\begin{equation}
	\int_0^{T_0} \cos(k \omega_0 t) dt =
	\begin{cases}
		T_0,& k=0\\
		0,& k \neq 0
	\end{cases}
\end{equation}

\textbf{Follows:}

\[
	\int_0^{T_0} \cos(k \omega_0 t) \cos(n \omega_0 t) dt 
	= \frac{1}{2} \int_0^{T_0} \left[ \cos\left((k-n)\omega_0 t\right) + \cos\left((k+n)\omega_0 t\right)\right] dt
\]


Case $k \neq n$:

\[
	\frac{1}{2} \int_0^{T_0} \left[ \cos\left(a \omega_0 t\right) + \cos\left(b \omega_0 t\right)\right] dt
	= \frac{1}{2} (0 + 0)
	= 0
\]

Case $k = n \neq 0$:

\[
	\frac{1}{2} \int_0^{T_0} \left[ \cos\left(0\right) + \cos\left(2k\omega_0 t\right)\right] dt
	= \frac{1}{2} T_0 + 0
	= \frac{T_0}{2}
\]

Case $k = n = 0$:

\[
	\frac{1}{2} \int_0^{T_0} \left[ \cos\left(0\right) + \cos\left(0\right)\right] dt
	= \frac{2}{2} T_0
	= T_0
\]

